crypto_hst/ec/Hacl.EC.Curve25519.Ladder.fst
@@ -31,7 +31,6 @@ module H128  = Hacl.UInt128
 // Will be specified using the bitwise operators' semantics
 val mk_mask: x:s8 -> Tot (y:s64(* {v y < pow2 platform_size /\ (Hacl.UInt8.v x = 0 ==> v y = 0) /\ (Hacl.UInt8.v x = 1 ==> v y = pow2 platform_size - 1)} *))
 let mk_mask x =
-  (* admit(); // OK *)
   let y = Hacl.Cast.sint8_to_sint64 x in
   H64 (Hacl.Cast.uint64_to_sint64 0uL -%^ y)
 
@@ -47,11 +46,11 @@ type distinct2 (n:bytes) (p:point) =
 
 #reset-options "--initial_fuel 0 --max_fuel 0 --z3timeout 5"
 
-val small_step_exit: 
-  two_p:point -> two_p_plus_q:point{distinct two_p two_p_plus_q /\ same_frame_2 two_p two_p_plus_q} -> 
-  p:point{distinct p two_p /\ distinct p two_p_plus_q /\ same_frame_2 two_p_plus_q p} -> 
-  p_plus_q:point{distinct p_plus_q two_p /\ distinct p_plus_q two_p_plus_q /\ distinct p_plus_q p /\ same_frame_2 p p_plus_q} -> 
-  q:point{distinct q two_p /\ distinct q two_p_plus_q /\ distinct q p /\ distinct q p_plus_q} -> 
+val small_step_exit:
+  two_p:point -> two_p_plus_q:point{distinct two_p two_p_plus_q /\ same_frame_2 two_p two_p_plus_q} ->
+  p:point{distinct p two_p /\ distinct p two_p_plus_q /\ same_frame_2 two_p_plus_q p} ->
+  p_plus_q:point{distinct p_plus_q two_p /\ distinct p_plus_q two_p_plus_q /\ distinct p_plus_q p /\ same_frame_2 p p_plus_q} ->
+  q:point{distinct q two_p /\ distinct q two_p_plus_q /\ distinct q p /\ distinct q p_plus_q} ->
   n:erased nat -> byte:s8 ->
   scalar:erased nat(* {reveal n = reveal scalar * (pow2 8) + (S8.v byte / (pow2 (8-8)))} *) ->
   Stack unit
@@ -68,34 +67,33 @@ val small_step_exit:
        // Formula_0 replaces (scalar * pow2 8 + byte)
        (* /\ (nTimesQ  (formula_0 scalar byte) (pointOf h0 q) h1 two_p two_p_plus_q) *)
 let small_step_exit pp ppq p pq q n byte scalar =
-  (* admit(); // OK *)
   (* let h0 = HST.get() in *)
   Hacl.EC.Curve25519.PPoint.copy2 pp ppq p pq;
   (* let h1 = HST.get() in *)
   (* distinct_lemma q p; distinct_lemma q pq; distinct_lemma q pp; distinct_lemma q ppq; *)
   (* let s = (erefs pp +*+ erefs ppq +*+ erefs p +*+ erefs pq) in *)
   (* cut(modifies (reveal s) h0 h1); *)
-  (* admitP(True /\ FStar.TSet.intersect (reveal s) (refs q) = !{}); *)
+  (* ad(True /\ FStar.TSet.intersect (reveal s) (refs q) = !{}); *)
   (* on_curve_lemma h0 h1 q (erefs pp +*+ erefs ppq +*+ erefs p +*+ erefs pq); *)
   (* cut(onCurve h1 q);  *)
   (* cut(nTimesQ (hide (reveal scalar * pow2 8 + (S8.v byte / pow2 (8-8)))) (pointOf h0 q) h0 p pq);  *)
   ()
   (* helper_lemma_1 scalar byte *)
 
-let same_ref (p:point) = as_ref (get_x p) == as_ref (get_y p) /\ as_ref (get_y p) == as_ref (get_z p)
-let distinct_ref (p:point) (p':point) = same_ref p /\ same_ref p' /\ as_ref (get_x p) =!= as_ref (get_x p')
+let lemma_helper_0 r s h0 h1 h2 h3 : Lemma
+  (requires (HS.modifies_ref r s h0 h1 /\ HS.modifies_ref r s h1 h2 /\ HS.modifies_ref r s h2 h3))
+  (ensures  (HS.modifies_ref r s h0 h3))
+  = ()
 
-
-(* TODO - WIP *)
 #reset-options "--initial_fuel 0 --max_fuel 0 --z3timeout 20"
 
-val small_step_core: 
-   two_p:point -> two_p_plus_q:point{distinct two_p two_p_plus_q /\ same_frame_2 two_p two_p_plus_q} -> 
+val small_step_core:
+   two_p:point -> two_p_plus_q:point{distinct two_p two_p_plus_q /\ same_frame_2 two_p two_p_plus_q} ->
    p:point{distinct two_p p /\ distinct two_p_plus_q p /\ same_frame_2 two_p_plus_q p} ->
-   p_plus_q:point{distinct two_p p_plus_q /\ distinct two_p_plus_q p_plus_q /\ distinct p_plus_q p /\ same_frame_2 p p_plus_q} -> 
+   p_plus_q:point{distinct two_p p_plus_q /\ distinct two_p_plus_q p_plus_q /\ distinct p_plus_q p /\ same_frame_2 p p_plus_q} ->
    q:point{same_frame q /\ frame_of q <> frame_of p
-   (* distinct q two_p /\ distinct q two_p_plus_q /\ distinct q p /\ distinct q p_plus_q *)} -> 
-   n:erased nat -> ctr:u32{U32.v ctr<8} -> byt:s8 -> scalar:erased nat(* {reveal n = reveal scalar * (pow2 (w ctr)) + (S8.v byt / (pow2 (8-w ctr)))} *) -> 
+   (* distinct q two_p /\ distinct q two_p_plus_q /\ distinct q p /\ distinct q p_plus_q *)} ->
+   n:erased nat -> ctr:u32{U32.v ctr<8} -> byt:s8 -> scalar:erased nat(* {reveal n = reveal scalar * (pow2 (w ctr)) + (S8.v byt / (pow2 (8-w ctr)))} *) ->
    Stack unit
      (requires (fun h -> live h two_p /\ live h two_p_plus_q /\ live h p /\ live h q /\ live h p_plus_q))
      (ensures (fun h0 _ h1 -> live h1 two_p /\ live h1 two_p_plus_q /\ live h1 p /\ live h1 p_plus_q
@@ -113,24 +111,25 @@ val small_step_core:
      (*   /\ (nTimesQ  (formula_2 (reveal n) (nth_bit byt ctr)) (pointOf h0 q) h1 two_p two_p_plus_q) *)
      (* )) *)
 let small_step_core pp ppq p pq q n ctr b scalar =
-  (* admit(); // TODO *)
   (* let h0 = HST.get() in *)
   (* distinct_commutative p pq; *)
   let bit = nth_bit b ctr in
   let mask = mk_mask bit in
   (* cut (v mask = pow2 platform_size - 1 \/ v mask = 0);  *)
   let h0 = HST.get() in
-  swap_conditional p pq mask; 
+  swap_conditional p pq mask;
   let h1 = HST.get() in assume (live h1 pp /\ live h1 ppq /\ live h1 q);
   (* let h = HST.get() in *)
   (* small_step_core_lemma_1 h0 h pp ppq p pq q; *)
   Hacl.EC.Curve25519.AddAndDouble.double_and_add pp ppq p pq q;
   let h2 = HST.get() in
   (* let h2 = HST.get() in *)
-  swap_conditional pp ppq mask; 
+  swap_conditional pp ppq mask;
   let h3 = HST.get() in assume (live h3 p /\ live h3 pq /\ live h3 q);
   Hacl.EC.Curve25519.AddAndDouble.lemma_helper_2 (frame_of p) h0 h1 (refs p ++ refs pq) (refs pp ++ refs ppq ++ refs p ++ refs pq);
   Hacl.EC.Curve25519.AddAndDouble.lemma_helper_2 (frame_of p) h2 h3 (refs pp ++ refs ppq) (refs pp ++ refs ppq ++ refs p ++ refs pq);
+  lemma_helper_0 (frame_of p) (refs pp ++ refs ppq ++ refs p ++ refs pq) h0 h1 h2 h3;
+  ()
   (* lemma_5 scalar b ctr; *)
   (* let h1 = HST.get() in *)
   (* assert ((live h2 p) /\ (live h2 pq) /\ (onCurve h2 q));  *)
@@ -147,12 +146,11 @@ let small_step_core pp ppq p pq q n ctr b scalar =
   (* cut (bit == uint8_to_sint8 1uy ==> ((pointOf h1 pp) = (pointOf h2 ppq) /\ (pointOf h1 ppq) = (pointOf h2 pp)));  *)
   (* cut (nTimesQ n (pointOf h0 q) h0 p pq);  *)
   (* small_step_core_lemma_3 h0 h h2 h1 pp ppq p pq q n ctr b scalar *)
-  ()
 
-val small_step: two_p:point -> two_p_plus_q:point{distinct two_p two_p_plus_q} ->
-   p:point{distinct p two_p /\ distinct p two_p_plus_q} ->
-   p_plus_q:point{distinct p_plus_q two_p /\ distinct p_plus_q two_p_plus_q /\ distinct p_plus_q p} ->
-   q:point{distinct q two_p /\ distinct q two_p_plus_q /\ distinct q p /\ distinct q p_plus_q} ->
+val small_step: two_p:point -> two_p_plus_q:point{distinct two_p two_p_plus_q /\ same_frame_2 two_p two_p_plus_q} ->
+   p:point{distinct p two_p /\ distinct p two_p_plus_q /\ same_frame_2 two_p_plus_q p} ->
+   p_plus_q:point{distinct p_plus_q two_p /\ distinct p_plus_q two_p_plus_q /\ distinct p_plus_q p /\ same_frame_2 p p_plus_q} ->
+   q:point{same_frame q /\ frame_of q <> frame_of p} ->
    n:erased nat -> ctr:u32{U32.v ctr<=8} -> b:s8 ->
    scalar:erased nat(* {reveal n = reveal scalar * (pow2 (w ctr)) + (S8.v b / (pow2 (8-w ctr)))} *) -> Stack unit
      (requires (fun h -> live h two_p /\ live h two_p_plus_q /\ live h p /\ live h q /\ live h p_plus_q))
@@ -168,43 +166,53 @@ val small_step: two_p:point -> two_p_plus_q:point{distinct two_p two_p_plus_q} -
      (*   /\ (nTimesQ  (formula_0 scalar b) (pointOf h0 q) h1 p p_plus_q) *)
      (* )) *)
 let rec small_step pp ppq p pq q n ctr b scalar =
-  (* admit(); // OK *)
   if U32 (8ul =^ ctr) then begin
     (* lemma_9 ctr; *)
     (* helper_lemma_1 n b;  *)
     ()
   end
   else begin
-    (* let h0 = HST.get() in *)
+    let h0 = HST.get() in
     (* lemma_0 ctr 8; *)
     small_step_core pp ppq p pq q n ctr b scalar;
-    (* let h1 = HST.get() in *)
+    let h1 = HST.get() in
     let bit = nth_bit b ctr in
     (* cut (nTimesQ (formula_1 n bit) (pointOf h0 q) h1 pp ppq); *)
     (* lemma_10 scalar ctr b; *)
     // Replaces a missing definition of the euclidian division
-    (* admitP (True /\ 2*reveal n+S8.v bit = reveal scalar * (pow2 (w ctr+1)) + (S8.v b / pow2 (8 - (w ctr+1)))); *)
+    (* admiP (True /\ 2*reveal n+S8.v bit = reveal scalar * (pow2 (w ctr+1)) + (S8.v b / pow2 (8 - (w ctr+1)))); *)
     (* cut (w ctr+1 <= 8 /\ True); *)
     (* assert (onCurve h1 pp /\ onCurve h1 ppq /\ live h1 p /\ live h1 pq); *)
     swap_both pp ppq p pq;
-    (* let h2 = HST.get() in *)
+    let h2 = HST.get() in
     (* assert (Math.Curve.equal (pointOf h2 p) (pointOf h1 pp) /\ Math.Curve.equal (pointOf h2 pq) (pointOf h1 ppq)); *)
     (* small_step_lemma_1 h0 h1 h2 pp ppq p pq q; *)
     (* formula_lemma n bit;  *)
     (* assert(nTimesQ (eformula_2 n bit) (pointOf h2 q) h2 p pq); *)
-    small_step pp ppq p pq q (hide 0(* eformula_2 n bit *)) (U32 (ctr+^1ul)) b scalar
-    (* let h3 = HST.get() in *)
+    small_step pp ppq p pq q (hide 0(* eformula_2 n bit *)) (U32 (ctr+^1ul)) b scalar;
+    let h3 = HST.get() in
     (* small_step_lemma_2 h0 h1 h2 h3 pp ppq p pq q *)
+    lemma_helper_0 (frame_of p) (refs pp ++ refs ppq ++ refs p ++ refs pq) h0 h1 h2 h3;
+    ()
   end
 
+#reset-options "--z3timeout 20 --initial_fuel 0 --max_fuel 0"
+
+
+let lemma_helper_1 r s h0 h1 h2 : Lemma
+  (requires (HS.modifies_ref r s h0 h1 /\ HS.modifies_ref r s h1 h2))
+  (ensures  (HS.modifies_ref r s h0 h2))
+  = ()
+
 val big_step:
-  n:bytes -> pp:point{distinct2 n pp} -> ppq:point{distinct2 n ppq /\ distinct pp ppq} ->
-   p:point{distinct2 n p /\ distinct p pp /\ distinct p ppq} ->
-   pq:point{distinct2 n pq /\ distinct pq pp /\ distinct pq ppq /\ distinct pq p} ->
-   q:point{distinct2 n q /\ distinct q pp /\ distinct q ppq /\ distinct q p /\ distinct q pq} ->
-   ctr:u32{U32.v ctr<=bytes_length} -> STL unit
-     (requires (fun h -> live h pp /\ live h ppq /\ live h p /\ live h q /\ live h pq))
-     (ensures (fun h0 _ h1 -> live h1 pp /\ live h1 ppq /\ live h1 p /\ live h1 pq
+  n:bytes{length n >= 32} -> pp:point{distinct2 n pp} ->
+  ppq:point{distinct2 n ppq /\ distinct pp ppq /\ same_frame_2 pp ppq /\ frame_of pp <> frameOf n} ->
+  p:point{distinct2 n p /\ distinct p pp /\ distinct p ppq /\ same_frame_2 ppq p} ->
+  pq:point{distinct2 n pq /\ distinct pq pp /\ distinct pq ppq /\ distinct pq p /\ same_frame_2 p pq} ->
+  q:point{distinct2 n q /\ same_frame q /\ frame_of p <> frame_of q} ->
+  ctr:u32{U32.v ctr<=bytes_length} -> STL unit
+    (requires (fun h -> B.live h n /\ live h pp /\ live h ppq /\ live h p /\ live h q /\ live h pq))
+    (ensures (fun h0 _ h1 -> live h1 pp /\ live h1 ppq /\ live h1 p /\ live h1 pq
        /\ HS.modifies_one (frame_of p) h0 h1
        /\ HS.modifies_ref (frame_of p) (refs pp ++ refs ppq ++ refs p ++ refs pq) h0 h1 ))
     (* (requires (fun h -> live h pp /\ live h ppq /\ onCurve h p /\ onCurve h pq /\ onCurve h q *)
@@ -215,62 +223,118 @@ val big_step:
     (*   /\ nTimesQ (formula_4 h0 n (w ctr)) (pointOf h0 q) h0 p pq *)
     (*   /\ nTimesQ (hide (valueOfBytes h0 n)) (pointOf h0 q) h1 p pq  )) *)
 let rec big_step n pp ppq p pq q ctr =
-  (* admit(); // OK modulo *)
-  (* let h0 = HST.get() in *)
+  let h0 = HST.get() in
   if U32 (blength =^ ctr) then () (* assume(reveal (formula_4 h0 n bytes_length) = valueOfBytes h0 n) *)
   else begin
     (* assume(bytes_length-1-w ctr>=0 /\ bytes_length-w ctr-1>=0); *)
     let byte = index n (U32 (blength-^1ul-^ctr)) in
     (* let m = formula_4 h0 n (w ctr) in *)
     // Replaces missing euclidian definitions in F*
-    (* admitP(reveal m = reveal m * pow2 0 + (S8.v byte / pow2 (8-0)) /\ True); *)
+    (* admiP(reveal m = reveal m * pow2 0 + (S8.v byte / pow2 (8-0)) /\ True); *)
     small_step pp ppq p pq q (hide 0)(* m *) 0ul byte (hide 0)(* m *);
-    (* let h1 = HST.get() in *)
+    let h1 = HST.get() in assert(live h1 q);
     (* big_step_lemma_1 h0 h1 n pp ppq p pq q ctr byte; *)
-    big_step n pp ppq p pq q (U32 (ctr +^ 1ul))
-    (* let h2 = HST.get() in *)
+    big_step n pp ppq p pq q (U32 (ctr +^ 1ul));
+    let h2 = HST.get() in
+    lemma_helper_1 (frame_of p) (refs pp ++ refs ppq ++ refs p ++ refs pq) h0 h1 h2;
+    ()
     (* big_step_lemma_2 h0 h1 h2 n pp ppq p pq q (w ctr) byte *)
   end
 
+#reset-options "--z3timeout 20 --initial_fuel 0 --max_fuel 0"
+
+private val init_points: q:point{same_frame q} -> tmp:bigint{length tmp = 66 /\ frameOf tmp <> frame_of q} -> Stack unit
+  (requires (fun h -> B.live h tmp /\ live h q))
+  (ensures  (fun h0 _ h1 -> B.live h1 tmp
+    /\ HS.modifies_one (frameOf tmp) h0 h1
+    /\ HS.modifies_ref (frameOf tmp) (arefs (only tmp)) h0 h1))
+let init_points q tmp =
+  let p_x = sub tmp 34ul 5ul in
+  let p_y = sub tmp 39ul 5ul in
+  let p_z = sub tmp 44ul 5ul in
+
+  let inf_x = sub tmp 49ul 6ul in
+  let h0 = HST.get() in
+  blit (get_x q) 0ul p_x 0ul nlength;
+  blit (get_y q) 0ul p_y 0ul nlength;
+  blit (get_z q) 0ul p_z 0ul nlength;
+  upd inf_x 0ul (Hacl.Cast.uint64_to_sint64 1uL);
+  let h1 = HST.get() in
+  assert(modifies_1 tmp h0 h1);
+  Hacl.EC.Curve25519.AddAndDouble.lemma_helper_0 h0 h1 tmp;
+  ()
+
+#reset-options "--z3timeout 20 --initial_fuel 0 --max_fuel 0"
+
+let lemma_helper_2 hinit h0 h1 h2 hfin r : Lemma
+  (requires (fresh_frame hinit h0 /\ HS.modifies_one h0.tip h0 h1 /\ HS.modifies_one r h1 h2
+    /\ popped h2 hfin /\ r `HS.is_in` hinit.h
+    /\ equal_domains hinit hfin))
+  (ensures  (HS.modifies_one r hinit hfin))
+  = assert(Set.subset (Map.domain hinit.h) (Map.domain hfin.h))
+
+
+#reset-options "--z3timeout 100 --initial_fuel 0 --max_fuel 0"
+
 val montgomery_ladder:
-  res:point -> n:bytes{distinct2 n res} -> q:point{distinct2 n q /\ distinct res q} ->
-  Stack unit
-    (requires (fun h -> live h res /\ live h q))
+  res:point{same_frame res} -> n:bytes{distinct2 n res /\ frame_of res <> frameOf n /\ length n >= 32} ->
+  q:point{same_frame q /\ frame_of q <> frame_of res /\ frame_of q <> frameOf n} -> Stack unit
+    (requires (fun h -> live h res /\ live h q /\ B.live h n))
       (* live h res /\ onCurve h q )) *)
     (ensures (fun h0 _ h1 -> live h1 res
-      /\ modifies_3 (get_x res) (get_y res) (get_z res) h0 h1))
+      /\ HS.modifies_one (frame_of res) h0 h1
+      /\ HS.modifies_ref (frame_of res) (refs res) h0 h1
+      /\ prop_2 h0 h1 res))
+    (* /\ modifies_3 (get_x res) (get_y res) (get_z res) h0 h1)) *)
     (* live h0 res /\ onCurve h0 q /\ onCurve h1 res *)
     (*   (\* /\ (modifies (refs res) h0 h1)  *\) *)
     (*   /\ (pointOf h1 res = (valueOfBytes h0 n +* (pointOf h0 q)))  )) *)
 let montgomery_ladder res n q =
+  let hinit = HST.get() in
   push_frame();
+
   // Build 'storage' empty but 'live' points
   let nlp1 = U32 (nlength +^ 1ul) in
-  let two_p_x = create (Hacl.Cast.uint64_to_sint64 0uL) nlp1 in
-  let two_p_y = create (Hacl.Cast.uint64_to_sint64 0uL) nlength in
-  let two_p_z = create (Hacl.Cast.uint64_to_sint64 0uL) nlp1 in
+  let tot_len = 66ul in
+  let h0 = HST.get() in
+  let tmp = create (Hacl.Cast.uint64_to_sint64 0uL) tot_len in
+  let two_p_x = sub tmp 0ul 6ul  in
+  let two_p_y = sub tmp 6ul 5ul in
+  let two_p_z = sub tmp 11ul 6ul in
+
+  let two_p_plus_q_x = sub tmp 17ul 6ul in
+  let two_p_plus_q_y = sub tmp 23ul 5ul in
+  let two_p_plus_q_z = sub tmp 28ul 6ul in
+
+  let p_x = sub tmp 34ul 5ul in
+  let p_y = sub tmp 39ul 5ul in
+  let p_z = sub tmp 44ul 5ul in
+
+  let inf_x = sub tmp 49ul 6ul in
+  let inf_y = sub tmp 55ul 5ul in
+  let inf_z = sub tmp 60ul 6ul in
+
   let two_p =  make two_p_x two_p_y two_p_z in
-  (* cut(distinct two_p q); *)
-  let two_p_plus_q_x = create (Hacl.Cast.uint64_to_sint64 0uL) nlp1 in
-  let two_p_plus_q_y = create (Hacl.Cast.uint64_to_sint64 0uL) nlength in
-  let two_p_plus_q_z = create (Hacl.Cast.uint64_to_sint64 0uL) nlp1 in
   let two_p_plus_q = make two_p_plus_q_x two_p_plus_q_y two_p_plus_q_z in
-  (* cut(distinct two_p_plus_q two_p /\ distinct two_p_plus_q q); *)
-  // Copy of the 'q' point
-  let p_x = create (Hacl.Cast.uint64_to_sint64 0uL) nlength in
-  blit (get_x q) 0ul p_x 0ul nlength;
-  let p_y = create (Hacl.Cast.uint64_to_sint64 0uL) nlength in
-  blit (get_y q) 0ul p_y 0ul nlength;
-  let p_z = create (Hacl.Cast.uint64_to_sint64 0uL) nlength in
-  blit (get_z q) 0ul p_z 0ul nlength;
   let p = make p_x p_y p_z in
-  // Point at infinity
-  let inf_x = create (Hacl.Cast.uint64_to_sint64 0uL) nlp1 in
-  upd inf_x 0ul (Hacl.Cast.uint64_to_sint64 1uL);
-  let inf_y = create (Hacl.Cast.uint64_to_sint64 0uL) nlength in
-  let inf_z = create (Hacl.Cast.uint64_to_sint64 0uL) nlp1 in
   let inf = make inf_x inf_y inf_z in
-  // Perform scalar multiplication by the content of 'n'
+  let h = HST.get() in
+
+  let h1 = HST.get() in
+  init_points q tmp;
+  let h2 = HST.get() in
+  cut (HS.modifies_one (frameOf tmp) h1 h2);
   big_step n two_p two_p_plus_q inf p q 0ul;
+  let h3 = HST.get() in
+  cut (HS.modifies_one (frameOf tmp) h2 h3);
   // Copy result to output
-  copy res two_p
+  copy res two_p;
+  let h4 = HST.get() in
+  cut (HS.modifies_one (frame_of res) h3 h4);
+
+  pop_frame();
+  let hfin = HST.get() in
+  assert(equal_domains hinit hfin);
+  lemma_reveal_modifies_0 h0 h1;
+  lemma_helper_2 hinit h0 h3 h4 hfin (frame_of res);
+  ()
